Making progress towards defining decoders as the inverse of encoders.

src/Boolify/src/CoderScript.sml
@@ -3,16 +3,27 @@
 (*===========================================================================*)
 
 (* Interactive mode
-app load ["rich_listTheory", "EncodeTheory", "DecodeTheory"];
+app load ["rich_listTheory", "EncodeTheory", "normalForms"];
 *)
 
 open HolKernel boolLib Parse bossLib pairTheory pairTools
      arithmeticTheory listTheory rich_listTheory EncodeTheory
-     mesonLib optionTheory DecodeTheory;
-
-val REVERSE = Tactical.REVERSE;
+     mesonLib optionTheory normalForms combinTheory;
 
 val _ = new_theory "Coder";
+
+infixr 0 ++ || <<;
+infix 1 >>;
+
+val op ++ = op THEN;
+val op >> = op THEN1;
+val op << = op THENL;
+val op || = op ORELSE;
+
+val Suff = Q_TAC SUFF_TAC;
+val Know = Q_TAC KNOW_TAC;
+
+val REVERSE = Tactical.REVERSE;
 
 (*---------------------------------------------------------------------------
      decode turns a decoding parser of type
@@ -27,34 +38,286 @@ val _ = new_theory "Coder";
 
 val decode_def = Define `decode f = FST o THE o f`;
 
-val domain_exists = store_thm
-  ("domain_exists",
-   ``?d. !f x. x IN d f = ?y. f x = SOME (y, [])``,
-   Q.EXISTS_TAC `\f x. ?y. f x = SOME (y, [])` THEN
+local
+  val th =prove
+  (``?d. !f x. x IN d f = ?y. f x = SOME (y, [])``,
+   Q.EXISTS_TAC `\f x. ?y. f x = SOME (y, [])` ++
    SIMP_TAC bool_ss [IN_DEF]);
+in
+  val domain_def =
+    Definition.new_specification ("domain_def", ["domain"], th);
+  val _ = add_const "domain";
+end;
 
-val domain_def =
-  Definition.new_specification
-  ("domain_def", ["domain"], domain_exists);
+(*---------------------------------------------------------------------------
+     Well-formed decoders.
+ ---------------------------------------------------------------------------*)
 
-val _ = add_const "domain";
+val wf_pdecoder_def = Define
+  `wf_pdecoder p (d : bool list -> ('a # bool list) option) =
+   !x.
+     if x IN p then (?a. !b c. (d b = SOME (x, c)) = (b = APPEND a c))
+     else !a b. ~(d a = SOME (x, b))`;
 
-val inverse_def = Define
-  `inverse e l =
-   if ?x t. l = APPEND (e x) t then SOME (@(x, t). l = APPEND (e x) t)
+(*---------------------------------------------------------------------------
+     Functions to transform well-formed encoders to well-formed decoders,
+     and vice versa.
+ ---------------------------------------------------------------------------*)
+
+val enc2dec_def = Define
+  `enc2dec p e (l : bool list) =
+   if ?x t. (x : 'a) IN p /\ (l = APPEND (e x) t)
+   then SOME (@(x, t). x IN p /\ (l = APPEND (e x) t))
    else NONE`;
 
-val inverse_none = prove
-  (``!e l. (inverse e l = NONE) = (!x t. ~(l = APPEND (e x) t))``,
-   RW_TAC std_ss [inverse_def] THEN
-   POP_ASSUM MP_TAC THEN
+val dec2enc_def = Define
+  `dec2enc (d : bool list -> ('a # bool list) option) x =
+   @l. d l = SOME (x, [])`;
+
+(*---------------------------------------------------------------------------
+     Proofs that the transformation functions are mutually inverse.
+ ---------------------------------------------------------------------------*)
+
+val enc2dec_none = store_thm
+  ("enc2dec_none",
+   ``!p e l.
+       (enc2dec p e l = NONE) = (!x t. x IN p ==> ~(l = APPEND (e x) t))``,
+   RW_TAC std_ss [enc2dec_def] ++
+   PROVE_TAC []);
+
+val enc2dec_some = store_thm
+  ("enc2dec_some",
+   ``!p e l x t.
+       wf_pencoder p e ==>
+       ((enc2dec p e l = SOME (x, t)) = x IN p /\ (l = APPEND (e x) t))``,
+   REVERSE (RW_TAC std_ss [enc2dec_def]) >> PROVE_TAC [] ++
+   ONCE_REWRITE_TAC [GSYM (ONCE_DEPTH_CONV ETA_CONV ``@p. q p``)] ++
+   SELECT_TAC ++
+   RW_TAC std_ss [UNCURRY] ++
+   Cases_on `p'` ++
+   EQ_TAC >>
+   (DISCH_THEN (fn th => POP_ASSUM MP_TAC THEN SUBST1_TAC th) ++
+    SIMP_TAC std_ss [] ++
+    DISCH_THEN MATCH_MP_TAC ++
+    PROVE_TAC [FST, SND]) ++
+   POP_ASSUM MP_TAC ++
+   MATCH_MP_TAC
+   (PROVE [] ``(z ==> x) /\ (y ==> z ==> t) ==> (x ==> y) ==> z ==> t``) ++
+   CONJ_TAC >> PROVE_TAC [FST, SND] ++
+   SIMP_TAC std_ss [] ++
+   REPEAT (DISCH_THEN STRIP_ASSUME_TAC) ++
+   Suff `q = x` >> PROVE_TAC [APPEND_11] ++
+   FULL_SIMP_TAC std_ss [wf_pencoder_def, RES_FORALL_DEF] ++
+   PROVE_TAC [IS_PREFIX_APPEND1, IS_PREFIX_APPEND2, IS_PREFIX_REFL]);
+
+val wf_enc2dec = store_thm
+  ("wf_enc2dec",
+   ``!p e. wf_pencoder p e ==> wf_pdecoder p (enc2dec p e)``,
+   RW_TAC std_ss [wf_pdecoder_def, enc2dec_some, RES_FORALL_DEF] ++
+   PROVE_TAC [APPEND_NIL]);
+
+val dec2enc_some = store_thm
+  ("dec2enc_some",
+   ``!p d x l.
+       wf_pdecoder p d ==>
+       ((dec2enc d x = l) /\ x IN p = (d l = SOME (x, [])))``,
+   RW_TAC std_ss [dec2enc_def] ++
+   SELECT_TAC ++
+   RW_TAC std_ss [] ++
+   EQ_TAC >>
+   (RW_TAC std_ss [] ++
+    Q.PAT_ASSUM `X ==> Y` MATCH_MP_TAC ++
+    FULL_SIMP_TAC std_ss [wf_pdecoder_def, RES_FORALL_DEF] ++
+    PROVE_TAC [APPEND_NIL]) ++
+   POP_ASSUM MP_TAC ++
+   MATCH_MP_TAC
+   (PROVE [] ``(z ==> x) /\ (y ==> z ==> t) ==> (x ==> y) ==> z ==> t``) ++
+   CONJ_TAC >> PROVE_TAC [] ++
+   POP_ASSUM MP_TAC ++
+   SIMP_TAC std_ss [wf_pdecoder_def] ++
+   DISCH_THEN (MP_TAC o Q.SPEC `x`) ++
+   REVERSE (Cases_on `x IN p`) >> PROVE_TAC [] ++
+   ASM_REWRITE_TAC [] ++
+   DISCH_THEN (CHOOSE_THEN MP_TAC) ++
    RW_TAC std_ss []);
 
-(*   
-val inverse_some = prove
-  (``!e l x t.
-       wf_encoder e ==>
-       ((inverse e l = SOME (x, t)) = (l = APPEND (e x) t))``,
+val decode_dec2enc = store_thm
+  ("decode_dec2enc",
+   ``!p d x.
+       wf_pdecoder p d /\ x IN p ==> (d (dec2enc d x) = SOME (x, []))``,
+   PROVE_TAC [dec2enc_some]);
+
+val decode_dec2enc_append = store_thm
+  ("decode_dec2enc_append",
+   ``!p d x t.
+       wf_pdecoder p d /\ x IN p ==>
+       (d (APPEND (dec2enc d x) t) = SOME (x, t))``,
+   RW_TAC std_ss [] ++
+   MP_TAC (Q.SPECL [`p`, `d`, `x`] decode_dec2enc) ++
+   RW_TAC std_ss [] ++
+   FULL_SIMP_TAC std_ss [wf_pdecoder_def] ++
+   Q.PAT_ASSUM `!x. P x` (MP_TAC o Q.SPEC `x`) ++
+   RW_TAC std_ss [] ++
+   RW_TAC std_ss [] ++
+   RES_TAC ++
+   RW_TAC std_ss [APPEND_NIL]);
+
+val wf_dec2enc = store_thm
+  ("wf_dec2enc",
+   ``!p d. wf_pdecoder p d ==> wf_pencoder p (dec2enc d)``,
+   RW_TAC std_ss [wf_pencoder_def, RES_FORALL_DEF] ++
+   MP_TAC (Q.SPECL [`p`, `d`] wf_pdecoder_def) ++
+   ASM_REWRITE_TAC [] ++
+   DISCH_THEN (fn th => MP_TAC (Q.SPEC `x` th) THEN MP_TAC (Q.SPEC `x'` th)) ++
+   RW_TAC std_ss [] ++
+   MP_TAC (Q.SPECL [`p`, `d`, `x`] decode_dec2enc) ++
+   MP_TAC (Q.SPECL [`p`, `d`, `x'`] decode_dec2enc) ++
+   RW_TAC std_ss [APPEND_NIL] ++
+   POP_ASSUM MP_TAC ++
+   POP_ASSUM MP_TAC ++
+   POP_ASSUM (CHOOSE_THEN MP_TAC o REWRITE_RULE [IS_PREFIX_APPEND]) ++
+   RW_TAC std_ss [GSYM APPEND_ASSOC] ++
+   POP_ASSUM (MP_TAC o Q.SPECL [`APPEND (dec2enc d x') l`, `[]`]) ++
+   POP_ASSUM (MP_TAC o Q.SPECL [`APPEND (dec2enc d x') l`, `l`]) ++
+   RW_TAC std_ss [APPEND_NIL]);
+
+val dec2enc_enc2dec = store_thm
+  ("dec2enc_enc2dec",
+   ``!p e x. wf_pencoder p e /\ x IN p ==> (dec2enc (enc2dec p e) x = e x)``,
+   RW_TAC std_ss [] ++
+   MP_TAC (Q.SPECL [`p`, `e`] wf_enc2dec) ++
+   RW_TAC std_ss [dec2enc_some] ++
+   MP_TAC (Q.SPECL [`p`, `enc2dec p e`, `x`, `e x`] dec2enc_some) ++
+   RW_TAC std_ss [enc2dec_some, APPEND_NIL]);
+
+val enc2dec_dec2enc = store_thm
+  ("enc2dec_dec2enc",
+   ``!p d. wf_pdecoder p d ==> (enc2dec p (dec2enc d) = d)``,
+   RW_TAC std_ss [] ++
+   MATCH_MP_TAC EQ_EXT ++
+   Q.X_GEN_TAC `l` ++
+   MP_TAC (Q.SPECL [`p`, `d`] wf_dec2enc) ++
+   RW_TAC std_ss [] ++
+   Cases_on `d l` <<
+   [RW_TAC std_ss [enc2dec_none] ++
+    STRIP_TAC ++
+    RW_TAC std_ss [] ++
+    Q.PAT_ASSUM `X = Y` MP_TAC ++
+    PROVE_TAC [NOT_SOME_NONE, decode_dec2enc_append],
+    Cases_on `x` ++
+    ASM_SIMP_TAC std_ss [enc2dec_some] ++
+    MATCH_MP_TAC (PROVE [] ``x /\ (x ==> y) ==> x /\ y``) ++
+    RW_TAC std_ss [] >> PROVE_TAC [wf_pdecoder_def] ++
+    MP_TAC (Q.SPECL [`p`, `d`] wf_pdecoder_def) ++
+    ASM_REWRITE_TAC [] ++
+    DISCH_THEN (MP_TAC o Q.SPEC `q`) ++
+    RW_TAC std_ss [] ++
+    RES_TAC ++
+    RW_TAC std_ss [APPEND_11] ++
+    Suff `d a = SOME (q, [])` >> PROVE_TAC [dec2enc_some] ++
+    RW_TAC std_ss [APPEND_NIL]]);
+
+val decode_encode = store_thm
+  ("decode_encode",
+   ``!p e x. wf_pencoder p e /\ x IN p ==> (decode (enc2dec p e) (e x) = x)``,
+   RW_TAC std_ss [] ++
+   Cases_on `enc2dec p e (e x)` >>
+   (POP_ASSUM MP_TAC ++
+    RW_TAC std_ss [enc2dec_none] ++
+    PROVE_TAC [APPEND_NIL]) ++
+   POP_ASSUM MP_TAC ++
+   Cases_on `x'` ++
+   SIMP_TAC std_ss [decode_def, o_THM] ++
+   RW_TAC std_ss [enc2dec_some] ++
+   MP_TAC (Q.SPECL [`p`, `e`] wf_pencoder_def) ++
+   RW_TAC std_ss [RES_FORALL_DEF] ++
+   Suff `IS_PREFIX (e x) (e q)` >> PROVE_TAC [] ++
+   PROVE_TAC [IS_PREFIX_APPEND]);
+
+val encode_decode = store_thm
+  ("encode_decode",
+   ``!p e l.
+       wf_pencoder p e /\ l IN domain (enc2dec p e) ==>
+       (e (decode (enc2dec p e) l) = l)``,
+   RW_TAC std_ss [domain_def, decode_def, o_THM] ++
+   RW_TAC std_ss [] ++
+   POP_ASSUM MP_TAC ++
+   RW_TAC std_ss [enc2dec_some, APPEND_NIL]);
+
+(* obsolete?
+val enc2dec_11 = store_thm
+  ("enc2dec_11",
+  ``!e f.
+       wf_encoder e /\ wf_encoder f /\ (enc2dec e = enc2dec f) ==> (e = f)``,
+   RW_TAC std_ss [] ++
+   MATCH_MP_TAC EQ_EXT ++
+   RW_TAC std_ss [] ++
+   MP_TAC (Q.SPECL [`e`, `e x`, `x`, `[]`] enc2dec_some) ++
+   RW_TAC std_ss [APPEND_NIL] ++
+   MP_TAC (Q.SPECL [`f`, `e x`, `x`, `[]`] enc2dec_some) ++
+   RW_TAC std_ss [APPEND_NIL]);
+*)
+
+(*---------------------------------------------------------------------------
+     We define decoders in terms of encoders.
+ ---------------------------------------------------------------------------*)
+
+val decode_bool_def = Define `decode_bool = enc2dec tot encode_bool`;
+
+val decode_list_def = Define
+  `decode_list d = enc2dec tot (encode_list (dec2enc d))`;
+
+(*---------------------------------------------------------------------------
+     decoders are well-formed and satisfy natural recursion equations.
+ ---------------------------------------------------------------------------*)
+
+val wf_decode_bool = store_thm
+  ("wf_decode_bool",
+   ``wf_pdecoder tot decode_bool``,
+   RW_TAC std_ss [decode_bool_def, wf_enc2dec, wf_encoder, wf_encode_bool]);
+
+val decode_encode_bool = store_thm
+  ("decode_encode_bool",
+   ``!x. decode decode_bool (encode_bool x) = x``,
+   RW_TAC std_ss
+   [decode_encode, decode_bool_def, wf_encoder, wf_encode_bool, tot_def]);
+
+val encode_decode_bool = store_thm
+  ("encode_decode_bool",
+   ``!l :: domain decode_bool. encode_bool (decode decode_bool l) = l``,
+   RW_TAC std_ss
+   [RES_FORALL_DEF, encode_decode, decode_bool_def, wf_encoder,
+    wf_encode_bool, tot_def]);
+
+val decode_bool = store_thm
+  ("decode_bool",
+   ``decode_bool l = case l of [] -> NONE || (h :: t) -> SOME (h, t)``,
+   REPEAT CASE_TAC ++
+   RW_TAC std_ss
+   [decode_bool_def, enc2dec_none, enc2dec_some, encode_bool_def,
+    APPEND, wf_encode_bool, wf_encoder, tot_def]);
+
+(* in progress
+val decode_list = store_thm
+  ("decode_list",
+   ``(decode_list d l =
+      case l of [] -> NONE
+      || (T :: t) ->
+         (case d t of NONE -> NONE
+          || SOME (x, t') ->
+             (case decode_list d t' of NONE -> NONE
+              || SOME (xs, t'') -> SOME (x :: xs, t'')))
+      || (F :: t) -> SOME ([], t))``,
+   (REPEAT CASE_TAC ++
+    RW_TAC std_ss [decode_list_def, enc2dec_none, tot_def]) <<
+   [Cases_on `x` ++
+    RW_TAC std_ss [encode_list_def, APPEND],
+    Cases_on `x` ++
+    RW_TAC std_ss [encode_list_def, APPEND, GSYM APPEND_ASSOC] ++
+    STRIP_TAC ++
+    RW_TAC std_ss []
+    
+); 
 *)
 
 val _ = export_theory ();
